Language.v
@@ -1,4 +1,12 @@
 Require Export Coq.Strings.String.
+Require Import Parity.
+Require Import AbstractBool.
+
+Inductive value : Type :=
+  | VNat : nat -> value
+  | VBool : bool -> value
+  | VAbstractBool : abstr_bool -> value
+  | VParity : parity -> value.
 
 Inductive aexp : Type :=
   | ANum : nat -> aexp
@@ -31,3 +39,10 @@ Notation "x '::=' a" :=
     (CAss x a) (at level 60) : com_scope.
 Notation "'try' c1 'catch' c2" :=
     (CTryCatch c1 c2) (at level 70) : com_scope.
+
+Definition plus_op (v1 v2 : value) : option value :=
+  match v1, v2 with
+  |  VNat x, VNat y =>  Some (VNat (plus x y))
+  |  VParity x, VParity y => Some (VParity (parity_plus x y))
+  | _, _ => None
+  end.
